Got earlier stuff to process.

veric/sim.v
@@ -47,16 +47,16 @@ Record CoreSemantics {G C M:Type} : Type :=
        forall ge m q m' q', corestep ge q m q' m' -> at_external q = None
 
   ; corestep_not_halted :
-       forall ge m q m' q', corestep ge q m q' m' -> safely_halted ge q m = None
+       forall ge m q m' q', corestep ge q m q' m' -> safely_halted ge q = None
 
   ; at_external_halted_excl :
-       forall ge q m, at_external q = None \/ safely_halted ge q m = None
+       forall ge q, at_external q = None \/ safely_halted ge q = None
   }.
 Implicit Arguments CoreSemantics [].
 
 (* Definition of multistepping. *)
 Section corestepN.
-  Context {G C M E:Type} (Sem:CoreSemantics G C M E) (ge:G).
+  Context {G C M E:Type} (Sem:CoreSemantics G C M) (ge:G).
 
   Fixpoint corestepN (n:nat) : C -> M -> C -> M -> Prop :=
     match n with
@@ -94,16 +94,21 @@ Section corestepN.
 End corestepN.
 
 (* A minimal preservation property we sometimes require.
- *)
-Definition mem_forward (m1 m2:mem) :=
+ 
+ Commented out when moving to forward_simulation eq/inj/ext *)
+(*Definition mem_forward (m1 m2:mem) :=
   (forall b, Mem.valid_block m1 b ->
       Mem.valid_block m2 b /\ 
        forall ofs, Mem.perm m1 b ofs Max = Mem.perm m2 b ofs Max).
-
-(* This predicate restricts what coresteps are allowed
+*)
+Definition mem_forward (m1 m2:mem) :=
+  (forall b, Mem.valid_block m1 b ->
+      Mem.valid_block m2 b /\ 
+       forall ofs p, Mem.perm m2 b ofs Max p -> Mem.perm m1 b ofs Max p).
+(*
+ This predicate restricts what coresteps are allowed
    to do.  Essentially, a corestep can only store, allocacte
-   and free, and must do so respecting permissions.
- *)
+   and free, and must do so respecting permissions.*) 
 Definition allowed_core_modification (m1 m2:mem) :=
   mem_forward m1 m2 /\
   (forall b ofs p,
@@ -118,7 +123,6 @@ Definition allowed_core_modification (m1 m2:mem) :=
     Mem.loadbytes m1 b ofs' n = Some vs ->
       (Mem.loadbytes m2 b ofs' n = Some vs) \/
       (exists ofs, ofs' <= ofs < ofs' + n /\ Mem.perm m1 b ofs Cur Writable)).
-
 
 (* The kinds of extensible semantics used by CompCert.  Memories are
    CompCert memories and external requests must contain external functions.
@@ -139,7 +143,7 @@ Record CompcertCoreSem {G C} :=
 Implicit Arguments CompcertCoreSem [ ].
 
 
-Lemma corestepN_fun (G C E:Type) (CSem:CompcertCoreSem G C E) :
+Lemma corestepN_fun (G C:Type) (CSem:CompcertCoreSem G C) :
   forall ge n c m c1 m1 c2 m2,
     corestepN CSem ge n c m c1 m1 ->
     corestepN CSem ge n c m c2 m2 ->
@@ -153,50 +157,6 @@ Proof.
   inv H0.
   eapply IHn; eauto.
 Qed.
-
- (* A "forward simulation structure" generalizes and axiomatizes
-    what it means for memories, values and addresses to "match".
-    We want to include the three matching relations used in
-    CompCert (equality, extension and injection) and allow
-    for composition in a natural way.
-
-    A key techincal trick is to use a parameterized type of "data"
-    which gives some witness to the match.  This generalized the
-    meminj used for memory injections and is crucial to get
-    composition to work.
-
-    There is a fair amount of overlap between the axioms relating
-    to matching addresses and the axioms relating to matching pointer
-    values.  This is because transitioning between the two is
-    nontrivial.  The transition requires translating between
-    unlimited precision integers and 32-bit integers.  This is only
-    sound if no addition overflow has occured, which we know only
-    if the pointer value corresponts to a valid pointer in
-    some appropriately matching memory.  So, similar axioms are
-    required on both sides of the boundary. 
-
-    The "big" lemmas at the end of the record give ways for
-    external function implementations to perform memory operations
-    in a controlled way.  Basically, the four major memory operations
-    are allowed.  When the same operation is called in related
-    memories with related arguments, one obtains related results.
-
-    BUG: currently, there is no way for external calls to change
-    permissions, which is necessary for, e.g., lock and unlock.
-    The memory model should probably expose a "change_perm"
-    operation which is intended only for use by external functions
-    and initilization.
-  *)
-
-(* Matching for lists of values with their types *)
-Inductive match_vals {D} (struct:ForwardSimulationStructure D) (d:D) :
-  (list typ) -> (list val) -> (list val) -> Prop :=
-| match_vals_nil : match_vals struct d nil nil nil
-| match_vals_cons : forall t ts v vs y ys,
-  match_val struct d t v y ->
-  match_vals struct d ts vs ys ->
-  match_vals struct d (t::ts) (v::vs) (y::ys).
-
 
 Inductive entry_points_compose: list (val*val*signature) -> list (val*val*signature) -> list (val*val*signature) -> Prop :=
 | EPC1: forall v1 v2 v3 sig r1 r2 r3, 
@@ -241,6 +201,7 @@ Hint Resolve
 
 (* First a forward simulation for passes which do not alter the memory
      layout at all. *)
+Module Sim_eq.
 Section Forward_simulation_equals. 
   Context {G1 C1 G2 C2:Type}
           {Sem1 : CompcertCoreSem G1 C1}
@@ -250,7 +211,7 @@ Section Forward_simulation_equals.
           {ge2:G2}
           {entry_points : list (val * val * signature)}.
 
-  Record forward_simulation_equals :=
+  Record Forward_simulation_equals :=
   { core_data:Type;
 
     match_core : core_data -> C1 -> C2 -> Prop;
@@ -281,12 +242,11 @@ Section Forward_simulation_equals.
       safely_halted Sem2 ge2 c2 = Some v;
 
     core_at_external : 
-      forall d st1 st2 args,
+      forall d st1 st2 e args,
         match_core d st1 st2 ->
         at_external Sem1 st1 = Some (e,args) ->
-        exists e2,
-          at_external Sem2 st2 = Some (e,args) /\
-          Forall2 Val.has_type args (sig_args (ef_sig e));
+        ( at_external Sem2 st2 = Some (e,args) /\
+          Forall2 Val.has_type args (sig_args (ef_sig e)) );
 
     core_after_external :
       forall d st1 st2 ret e args,
@@ -294,15 +254,18 @@ Section Forward_simulation_equals.
         at_external Sem1 st1 = Some (e,args) ->
         at_external Sem2 st2 = Some (e,args) ->
         Forall2 Val.has_type args (sig_args (ef_sig e)) ->
-        Val.has_type ret (proj_sig_res sig) ->
+        Val.has_type ret (proj_sig_res (ef_sig e)) ->
         exists st1', exists st2', exists d',
           after_external Sem1 ret st1 = Some st1' /\
           after_external Sem2 ret st2 = Some st2' /\
           match_core d' st1' st2'
   }.
-
 End Forward_simulation_equals. 
 
+Implicit Arguments Forward_simulation_equals [[G1] [C1] [G2] [C2]].
+End Sim_eq.
+
+Module Sim_inj.
 (* An axiom for passes that use memory injections. *)
 Section Forward_simulation_inject. 
   Context {G1 C1 G2 C2:Type}
@@ -313,7 +276,7 @@ Section Forward_simulation_inject.
           {ge2:G2}
           {entry_points : list (val * val * signature)}.
 
-  Record forward_simulation_inject := {
+  Record Forward_simulation_inject := {
     core_data : Type;
 
     match_state : core_data -> meminj -> C1 -> mem -> C2 -> mem -> Prop;
@@ -372,9 +335,10 @@ Section Forward_simulation_inject.
         Mem.inject j' m1' m2' ->
         val_inject j' ret1 ret2 ->
 
-        mem_unchanged_on (loc_unmapped j) m1 m1' ->
-        mem_unchanged_on (loc_out_of_reach j m1) m2 m2' ->
-        mem_forward m1 m1' ->
+        mem_unchanged_on (loc_unmapped j) m1 m1' ->  (*together, these 2 conditions say roughly that*)
+        mem_unchanged_on (loc_out_of_reach j m1) m2 m2' -> (* spill-locations didn't change*)
+
+        mem_forward m1 m1' ->  
         mem_forward m2 m2' ->
 
         Forall2 (Val.has_type) vals2 (sig_args (ef_sig e)) ->
@@ -386,7 +350,12 @@ Section Forward_simulation_inject.
           match_state cd' j' st1' m1' st2' m2'
     }.
 
-End ForwardSimulation_Inject.
+End Forward_simulation_inject.
+
+Implicit Arguments Forward_simulation_inject[[G1] [C1] [G2] [C2]].
+End Sim_inj.
+
+Module Sim_ext.
 
 (* Next, an axiom for passes that allow the memory to undergo extension. *)
 Section Forward_simulation_extends. 
@@ -398,7 +367,7 @@ Section Forward_simulation_extends.
           {ge2:G2}
           {entry_points : list (val * val * signature)}.
 
-  Record forward_simulation_extend := {
+  Record Forward_simulation_extends := {
     core_data : Type;
 
     match_state : core_data -> C1 -> mem -> C2 -> mem -> Prop;
@@ -451,10 +420,10 @@ Section Forward_simulation_extends.
 
         Forall2 Val.lessdef vals1 vals2 ->
         Forall2 (Val.has_type) vals2 (sig_args (ef_sig e)) ->
-      
         mem_forward m1 m1' ->
         mem_forward m2 m2' ->
-        mem_unchanged_on (loc_out_of_bounds m1) m2 m2' ->
+
+        mem_unchanged_on (loc_out_of_bounds m1) m2 m2' -> (*ie spill-locations didn't change*)
         Val.lessdef ret1 ret2 ->
         Mem.extends m1' m2' ->
 
@@ -465,7 +434,10 @@ Section Forward_simulation_extends.
           after_external Sem2 ret2 st2 = Some st2' /\
           match_state cd' st1' m1' st2' m2'
    }.
-End ForwardSimulation_Extend.
+End Forward_simulation_extends.
+
+Implicit Arguments Forward_simulation_extends [[G1] [C1] [G2] [C2]].
+End Sim_ext.
 
   (* An axiom stating that inject forward simulations compose *)
   Axiom forward_simulation_inject_inject_compose : forall
@@ -481,13 +453,13 @@ End ForwardSimulation_Extend.
     (entry_points12 : list (val*val*signature))
     (entry_points23 : list (val*val*signature))
 
-    (FSim12 : ForwardSimulation_inject Sem1 Sem2 ge1 ge2 entry_points12)
-    (FSim23 : ForwardSimulation_inject Sem2 Sem3 ge2 ge3 entry_points23)
+    (FSim12 : Sim_inj.Forward_simulation_inject Sem1 Sem2 ge1 ge2 entry_points12)
+    (FSim23 : Sim_inj.Forward_simulation_inject Sem2 Sem3 ge2 ge3 entry_points23)
 
     (entry_points13: list (val*val*signature))
     (EPC: entry_points_compose entry_points12 entry_points23 entry_points13),
 
-    ForwardSimulation_inject Sem1 Sem3 ge1 ge3 entry_points13.
+    Sim_inj.Forward_simulation_inject Sem1 Sem3 ge1 ge3 entry_points13.
 
   (* An axiom stating that extend_inject forward simulations compose *)
   Axiom forward_simulation_extend_inject_compose : forall
@@ -503,13 +475,13 @@ End ForwardSimulation_Extend.
     (entry_points12 : list (val*val*signature))
     (entry_points23 : list (val*val*signature))
 
-    (FSim12 : ForwardSimulation_extend Sem1 Sem2 ge1 ge2 entry_points12)
-    (FSim23 : ForwardSimulation_inject Sem2 Sem3 ge2 ge3 entry_points23)
+    (FSim12 : Sim_ext.Forward_simulation_extends Sem1 Sem2 ge1 ge2 entry_points12)
+    (FSim23 : Sim_inj.Forward_simulation_inject Sem2 Sem3 ge2 ge3 entry_points23)
 
     (entry_points13: list (val*val*signature))
     (EPC: entry_points_compose entry_points12 entry_points23 entry_points13),
 
-    ForwardSimulation_inject Sem1 Sem3 ge1 ge3 entry_points13.
+    Sim_inj.Forward_simulation_inject Sem1 Sem3 ge1 ge3 entry_points13.
 
   (* An axiom stating that equal inject forward simulations compose *)
   Axiom forward_simulation_equal_inject_compose : forall
@@ -525,15 +497,489 @@ End ForwardSimulation_Extend.
     (entry_points12 : list (val*val*signature))
     (entry_points23 : list (val*val*signature))
 
-    (FSim12 : ForwardSimulation_equal Sem1 Sem2 ge1 ge2 entry_points12)
-    (FSim23 : ForwardSimulation_inject Sem2 Sem3 ge2 ge3 entry_points23)
+    (FSim12 : Sim_eq.Forward_simulation_equals Sem1 Sem2 ge1 ge2 entry_points12)
+    (FSim23 : Sim_inj.Forward_simulation_inject Sem2 Sem3 ge2 ge3 entry_points23)
 
     (entry_points13: list (val*val*signature))
     (EPC: entry_points_compose entry_points12 entry_points23 entry_points13),
 
-    ForwardSimulation_inject Sem1 Sem3 ge1 ge3 entry_points13.
+    Sim_inj.Forward_simulation_inject Sem1 Sem3 ge1 ge3 entry_points13.
 
 End SIMULATIONS.
+
+Module Sim_proof <: SIMULATIONS.
+
+
+Lemma mem_forward_refl : forall m,
+  mem_forward m m.
+Proof.
+  repeat intro; auto.
+Qed.
+
+Lemma mem_forward_trans : forall m1 m2 m3,
+  mem_forward m1 m2 ->
+  mem_forward m2 m3 ->
+  mem_forward m1 m3.
+Proof.
+  repeat intro; auto.
+  apply H in H1. destruct H1.
+  apply H0 in H1. destruct H1.
+  split; auto.
+Qed.
+
+Lemma free_mem_forward :  forall m1 b lo hi m2,
+  Mem.free m1 b lo hi = Some m2 ->
+  mem_forward m1 m2.
+Proof.
+  repeat intro.
+  split.
+  eapply Mem.valid_block_free_1; eauto.
+  intros. eapply Mem.perm_free_3.  apply H. apply H1.
+Qed.
+
+Lemma store_mem_forward : forall chunk m1 b ofs v m2,
+  Mem.store chunk m1 b ofs v = Some m2 ->
+  mem_forward m1 m2.
+Proof.
+  repeat intro. split.
+  eapply Mem.store_valid_block_1; eauto.
+  intros.
+  admit.  (* likely true *)
+Qed.
+
+Lemma alloc_mem_forward : forall m1 b lo hi m2,
+  Mem.alloc m1 lo hi = (m2,b) ->
+  mem_forward m1 m2.
+Proof.
+  repeat intro. split.
+  eapply Mem.valid_block_alloc; eauto.
+  admit.  (* likely true *)
+Qed.
+
+
+Lemma allowed_core_modification_refl : forall m,
+  allowed_core_modification m m.
+Proof.
+  clear. intros.
+  hnf. split; auto.
+  apply mem_forward_refl.
+Qed.
+
+Lemma allowed_core_modification_trans : forall m1 m2 m3,
+  allowed_core_modification m1 m2 ->
+  allowed_core_modification m2 m3 ->
+  allowed_core_modification m1 m3.
+Proof.
+  intros. destruct H. destruct H0.
+  split.
+  eapply mem_forward_trans; eauto.
+  destruct H1; destruct H2.
+  split; intros.
+  specialize (H1 b ofs p H5).
+  destruct H1.
+  specialize (H2 b ofs p H1).
+  destruct H2; auto.
+  right. destruct H2; split; auto.
+  destruct H3. apply H3; auto.
+  apply Mem.perm_valid_block in H5. auto.
+  destruct H1.
+  right. split; auto.
+  repeat intro.
+  eapply H6.
+  destruct H4. eapply H4; eauto.
+  apply Mem.perm_valid_block in H5. 
+  apply H in H5. destruct H5; auto.
+  
+  split; intros.
+  destruct H3. destruct H4.
+  apply H3; auto.
+  apply H4; auto.
+  apply H in H5. destruct H5; auto.
+  destruct H3; destruct H4.
+  generalize H5; intros.
+  apply H6 in H5. destruct H5.
+  generalize H5; intros.
+  apply H7 in H5. destruct H5. auto.
+  destruct H5 as [ofs [? ?]].
+  right. exists ofs. split; auto.
+  apply H3; auto.
+  admit.  (* whatever *)
+  admit.  (* whatever *)
+Qed.
+
+Require Import Zwf.
+
+(*
+Lemma getN_clearN : forall n ofs' m1 b lo hi,
+  ofs' + n <= lo \/ hi <= ofs' ->
+  Mem.getN (nat_of_Z n) ofs' (Mem.clearN (Mem.mem_contents m1) b lo hi b) =
+  Mem.getN (nat_of_Z n) ofs' (Mem.mem_contents m1 b).
+Proof.
+  intro n.
+  induction n using (well_founded_induction (Zwf_well_founded 0)).
+  intros.
+  assert (n <= 0 \/ n > 0) by omega.
+  destruct H1.
+  replace (nat_of_Z n) with O. simpl. auto.
+  symmetry. apply nat_of_Z_neg. auto.
+  replace n with (1 + (n - 1)) by omega.
+  rewrite nat_of_Z_plus. 2: omega. 2: omega.
+  simpl. f_equal.
+  unfold Mem.clearN.
+  destruct (zeq b b).
+  destruct (zle lo ofs').
+  destruct (zlt ofs' hi).
+  elimtype False. omega.
+  simpl; auto. simpl; auto.
+  elim n0; auto.
+  apply H.
+  red. omega.
+  omega.
+Qed.
+*)
+
+Lemma free_allowed_core_mod : forall m1 b lo hi m2,
+  Mem.free m1 b lo hi = Some m2 ->
+  allowed_core_modification m1 m2.
+Proof.
+  intros. split.
+  eapply free_mem_forward; eauto.
+  split; intros.
+  unfold block in *.
+  assert 
+    ((b0 <> b \/ ofs < lo \/ hi <= ofs) \/
+     (b = b0 /\ lo <= ofs /\ ofs < hi)) by omega.
+  destruct H1.
+  left. eapply Mem.perm_free_1; eauto.
+  destruct H1; subst.
+  right. split.
+  apply Mem.free_range_perm in H.
+  apply H. auto.
+  intro. eapply Mem.perm_free_2; eauto.
+  split; intros.
+  eapply Mem.perm_free_3; eauto.
+  admit. (*whatever*)
+Qed.
+
+
+Lemma alloc_allowed_core_mod : forall m1 lo hi m2 b,
+  Mem.alloc m1 lo hi = (m2,b) ->
+  allowed_core_modification m1 m2.
+Proof.
+  intros. split.
+  eapply alloc_mem_forward; eauto.
+
+  split; intros.
+  left. eapply Mem.perm_alloc_1; eauto.
+  split; intros.
+  eapply Mem.perm_alloc_inv in H1; eauto.
+  destruct (zeq b0 b); subst; auto.
+  elimtype False. revert H0.
+  eapply Mem.fresh_block_alloc; eauto.
+  
+  left.
+  admit. (*whatever*)
+Qed.
+
+
+Lemma store_allowed_core_mod : forall m1 chunk v b ofs m2,
+  Mem.store chunk m1 b ofs v = Some m2 ->
+  allowed_core_modification m1 m2.
+Proof.
+  intros. split.
+  eapply store_mem_forward; eauto.
+
+  split; intros.
+  left. eapply Mem.perm_store_1; eauto.
+  split; intros.
+  eapply Mem.perm_store_2; eauto.
+  rename b0 into b'.
+  unfold block in *.
+  assert
+    ((b' <> b \/ n <= 0 \/ ofs' + n <= ofs \/ ofs + size_chunk chunk <= ofs') \/
+     (b' = b /\ 0 < n /\ ofs < ofs' + n /\ ofs' < ofs + size_chunk chunk)) by omega.
+  destruct H1.
+  left. erewrite Mem.loadbytes_store_other; eauto.
+  destruct H1; subst.
+  right.
+  apply Mem.store_valid_access_3 in H.
+  assert (ofs' <= ofs \/ ofs < ofs') by omega.
+  destruct H1.
+  exists ofs. split. omega.
+  apply H. destruct chunk; simpl; omega.
+  assert (ofs + size_chunk chunk < ofs' +  n \/ ofs' + n  <= ofs + size_chunk chunk) by omega.
+  destruct H3.
+  exists (ofs + size_chunk chunk - 1).
+  split. omega.
+  apply H.
+  destruct chunk; simpl in *; omega.
+  exists ofs'. split. omega.
+  apply H.
+  omega.
+Qed.
+
+Module Sim_eq.
+Section Forward_simulation_equals. 
+  Context {G1 C1 G2 C2:Type}
+          {Sem1 : CompcertCoreSem G1 C1}
+          {Sem2 : CompcertCoreSem G2 C2}
+
+          {ge1:G1}
+          {ge2:G2}
+          {entry_points : list (val * val * signature)}.
+
+  Record Forward_simulation_equals :=
+  { core_data:Type;
+
+    match_core : core_data -> C1 -> C2 -> Prop;
+    core_ord : C1 -> C1 -> Prop;
+    core_ord_wf : well_founded core_ord;
+
+    core_diagram : 
+      forall st1 m st1' m', corestep Sem1 ge1 st1 m st1' m' ->
+      forall d st2, match_core d st1 st2 ->
+        exists st2', exists d',
+          match_core d' st1' st2' /\
+          ((corestep_plus Sem2 ge2 st2 m st2' m') \/
+            corestep_star Sem2 ge2 st2 m st2' m' /\
+            core_ord st1' st1);
+
+    core_initial : forall v1 v2 sig,
+      In (v1,v2,sig) entry_points ->
+        forall vals,
+          Forall2 (Val.has_type) vals (sig_args sig) ->
+          exists cd, exists c1, exists c2,
+            make_initial_core Sem1 ge1 v1 vals = Some c1 /\
+            make_initial_core Sem2 ge2 v2 vals = Some c2 /\
+            match_core cd c1 c2;
+
+    core_halted : forall cd c1 c2 (v:int),
+      match_core cd c1 c2 ->
+      safely_halted Sem1 ge1 c1 = Some v ->
+      safely_halted Sem2 ge2 c2 = Some v;
+
+    core_at_external : 
+      forall d st1 st2 e args,
+        match_core d st1 st2 ->
+        at_external Sem1 st1 = Some (e,args) ->
+        ( at_external Sem2 st2 = Some (e,args) /\
+          Forall2 Val.has_type args (sig_args (ef_sig e)) );
+
+    core_after_external :
+      forall d st1 st2 ret e args,
+        match_core d st1 st2 ->
+        at_external Sem1 st1 = Some (e,args) ->
+        at_external Sem2 st2 = Some (e,args) ->
+        Forall2 Val.has_type args (sig_args (ef_sig e)) ->
+        Val.has_type ret (proj_sig_res (ef_sig e)) ->
+        exists st1', exists st2', exists d',
+          after_external Sem1 ret st1 = Some st1' /\
+          after_external Sem2 ret st2 = Some st2' /\
+          match_core d' st1' st2'
+  }.
+End Forward_simulation_equals. 
+
+Implicit Arguments Forward_simulation_equals [[G1] [C1] [G2] [C2]].
+End Sim_eq.
+
+Module Sim_inj.
+(* An axiom for passes that use memory injections. *)
+Section Forward_simulation_inject. 
+  Context {G1 C1 G2 C2:Type}
+          {Sem1 : CompcertCoreSem G1 C1}
+          {Sem2 : CompcertCoreSem G2 C2}
+
+          {ge1:G1}
+          {ge2:G2}
+          {entry_points : list (val * val * signature)}.
+
+  Record Forward_simulation_inject := {
+    core_data : Type;
+
+    match_state : core_data -> meminj -> C1 -> mem -> C2 -> mem -> Prop;
+    core_ord : C1 -> C1 -> Prop;
+    core_ord_wf : well_founded core_ord;
+
+    core_diagram : 
+      forall st1 m1 st1' m1', corestep Sem1 ge1 st1 m1 st1' m1' ->
+      forall cd st2 j m2,
+        match_state cd j st1 m1 st2 m2 ->
+        exists st2', exists m2', exists cd', exists j',
+          inject_incr j j' /\
+          inject_separated j j' m1 m2 /\
+          match_state cd' j' st1' m1' st2' m2' /\
+          ((corestep_plus Sem2 ge2 st2 m2 st2' m2') \/
+            corestep_star Sem2 ge2 st2 m2 st2' m2' /\
+            core_ord st1' st1);
+
+    core_initial : forall v1 v2 sig,
+      In (v1,v2,sig) entry_points ->
+        forall j vals vals' m1 m2,
+          Forall2 (val_inject j) vals vals' ->
+          Forall2 (Val.has_type) vals' (sig_args sig) ->
+          Mem.inject j m1 m2 ->
+          exists cd, exists c1, exists c2,
+            make_initial_core Sem1 ge1 v1 vals = Some c1 /\
+            make_initial_core Sem2 ge2 v2 vals' = Some c2 /\
+            match_state cd j c1 m1 c2 m2;
+
+    core_halted : forall cd j c1 m1 c2 m2 (v1:int),
+      match_state cd j c1 m1 c2 m2 ->
+      safely_halted Sem1 ge1 c1 = Some v1 ->
+        (safely_halted Sem2 ge2 c2 = Some v1 /\
+         Mem.inject j m1 m2); (*conjunct Mem.inject j m1 m2 could maybe deleted here?*)
+
+    core_at_external : 
+      forall cd j st1 m1 st2 m2 e vals1,
+        match_state cd j st1 m1 st2 m2 ->
+        at_external Sem1 st1 = Some (e,vals1) ->
+        exists vals2,
+          Mem.inject j m1 m2 /\
+          Forall2 (val_inject j) vals1 vals2 /\
+          Forall2 (Val.has_type) vals2 (sig_args (ef_sig e)) /\
+          at_external Sem2 st2 = Some (e,vals2);
+  
+    core_after_external :
+      forall cd j j' st1 st2 m1 m2 e vals1 vals2 ret1 ret2 m1' m2',
+        match_state cd j st1 m1 st2 m2 ->
+        Mem.inject j m1 m2 ->
+        at_external Sem1 st1 = Some (e,vals1) ->
+        at_external Sem2 st2 = Some (e,vals2) ->
+        Forall2 (val_inject j) vals1 vals2 ->
+      
+        inject_incr j j' ->
+        inject_separated j j' m1 m2 ->
+        Mem.inject j' m1' m2' ->
+        val_inject j' ret1 ret2 ->
+
+        mem_unchanged_on (loc_unmapped j) m1 m1' ->  (*together, these 2 conditions say roughly that*)
+        mem_unchanged_on (loc_out_of_reach j m1) m2 m2' -> (* spill-locations didn't change*)
+
+        mem_forward m1 m1' ->  
+        mem_forward m2 m2' ->
+
+        Forall2 (Val.has_type) vals2 (sig_args (ef_sig e)) ->
+        Val.has_type ret2 (proj_sig_res (ef_sig e)) ->
+
+        exists cd', exists st1', exists st2',
+          after_external Sem1 ret1 st1 = Some st1' /\
+          after_external Sem2 ret2 st2 = Some st2' /\
+          match_state cd' j' st1' m1' st2' m2'
+    }.
+
+End Forward_simulation_inject.
+
+Implicit Arguments Forward_simulation_inject[[G1] [C1] [G2] [C2]].
+End Sim_inj.
+
+Module Sim_ext.
+
+(* Next, an axiom for passes that allow the memory to undergo extension. *)
+Section Forward_simulation_extends. 
+  Context {G1 C1 G2 C2:Type}
+          {Sem1 : CompcertCoreSem G1 C1}
+          {Sem2 : CompcertCoreSem G2 C2}
+
+          {ge1:G1}
+          {ge2:G2}
+          {entry_points : list (val * val * signature)}.
+
+  Record Forward_simulation_extends := {
+    core_data : Type;
+
+    match_state : core_data -> C1 -> mem -> C2 -> mem -> Prop;
+    core_ord : C1 -> C1 -> Prop;
+    core_ord_wf : well_founded core_ord;
+
+    core_diagram : 
+      forall st1 m1 st1' m1', corestep Sem1 ge1 st1 m1 st1' m1' ->
+      forall cd st2 m2,
+        match_state cd st1 m1 st2 m2 ->
+        exists st2', exists m2', exists cd',
+          match_state cd' st1' m1' st2' m2' /\
+          ((corestep_plus Sem2 ge2 st2 m2 st2' m2') \/
+            corestep_star Sem2 ge2 st2 m2 st2' m2' /\
+            core_ord st1' st1);
+
+    core_initial : forall v1 v2 sig,
+      In (v1,v2,sig) entry_points ->
+        forall vals vals' m1 m2,
+          Forall2 Val.lessdef vals vals' ->
+          Forall2 (Val.has_type) vals' (sig_args sig) ->
+          Mem.extends m1 m2 ->
+          exists cd, exists c1, exists c2,
+            make_initial_core Sem1 ge1 v1 vals = Some c1 /\
+            make_initial_core Sem2 ge2 v2 vals' = Some c2 /\
+            match_state cd c1 m1 c2 m2;
+
+    core_halted : 
+      forall cd st1 m1 st2 m2 (v:int),
+        match_state cd st1 m1 st2 m2 ->
+        safely_halted Sem1 ge1 st1 = Some v ->
+          safely_halted Sem2 ge2 st2 = Some v /\
+          Mem.extends m1 m2;
+
+    core_at_external : 
+      forall cd st1 m1 st2 m2 e vals1,
+        match_state cd st1 m1 st2 m2 ->
+        at_external Sem1 st1 = Some (e,vals1) ->
+        exists vals2,
+          Mem.extends m1 m2 /\
+          Forall2 Val.lessdef vals1 vals2 /\
+          Forall2 (Val.has_type) vals2 (sig_args (ef_sig e)) /\
+          at_external Sem2 st2 = Some (e,vals2);
+
+    core_after_external :
+      forall cd st1 st2 m1 m2 e vals1 vals2 ret1 ret2 m1' m2',
+        match_state cd st1 m1 st2 m2 ->
+        at_external Sem1 st1 = Some (e,vals1) ->
+        at_external Sem2 st2 = Some (e,vals2) ->
+
+        Forall2 Val.lessdef vals1 vals2 ->
+        Forall2 (Val.has_type) vals2 (sig_args (ef_sig e)) ->
+        mem_forward m1 m1' ->
+        mem_forward m2 m2' ->
+
+        mem_unchanged_on (loc_out_of_bounds m1) m2 m2' -> (*ie spill-locations didn't change*)
+        Val.lessdef ret1 ret2 ->
+        Mem.extends m1' m2' ->
+
+        Val.has_type ret2 (proj_sig_res (ef_sig e)) ->
+
+        exists st1', exists st2', exists cd',
+          after_external Sem1 ret1 st1 = Some st1' /\
+          after_external Sem2 ret2 st2 = Some st2' /\
+          match_state cd' st1' m1' st2' m2'
+   }.
+End Forward_simulation_extends.
+
+Implicit Arguments Forward_simulation_extends [[G1] [C1] [G2] [C2]].
+End Sim_ext.
+
+  (* An axiom stating that inject forward simulations compose *)
+  Lemma forward_simulation_inject_inject_compose : forall
+    (G1 C1 G2 C2 G3 C3:Type)
+    (Sem1 : CompcertCoreSem G1 C1)
+    (Sem2 : CompcertCoreSem G2 C2)
+    (Sem3 : CompcertCoreSem G3 C3)
+
+    (ge1 : G1)
+    (ge2 : G2)
+    (ge3 : G3)
+
+    (entry_points12 : list (val*val*signature))
+    (entry_points23 : list (val*val*signature))
+
+    (FSim12 : Sim_inj.Forward_simulation_inject Sem1 Sem2 ge1 ge2 entry_points12)
+    (FSim23 : Sim_inj.Forward_simulation_inject Sem2 Sem3 ge2 ge3 entry_points23)
+
+    (entry_points13: list (val*val*signature))
+    (EPC: entry_points_compose entry_points12 entry_points23 entry_points13),
+
+    Sim_inj.Forward_simulation_inject Sem1 Sem3 ge1 ge3 entry_points13.
+  Proof.
+    intros. 
+  Qed.
 
 (* This module type states that forward simulations are sufficent
    to imply correctness with respect to the trace model of external
